\section*{Exercises for \ref{sec:2_1}}

\begin{Filesave}{solutions}
\solsection{Section~\ref{sec:2_1}}
\end{Filesave}

\begin{multicols}{2}
\begin{ex}
Find $a$, $b$, $c$, and $d$ if


\begin{enumerate}[label={\alph*.}]
\item 
$
\leftB \begin{array}{cc}
a & b \\
c & d
\end{array} \rightB = 
\leftB \begin{array}{cc}
c - 3d & -d \\
2a + d & a + b
\end{array} \rightB
$

\item 
$
\leftB \begin{array}{cc}
a - b & b - c \\
c - d & d - a
\end{array} \rightB = 2
\leftB \begin{array}{rr}
1 & 1 \\
-3 & 1
\end{array} \rightB
$

\item 
$
3 \leftB \begin{array}{c}
a \\
b
\end{array} \rightB + 2
\leftB \begin{array}{rr}
b \\
a
\end{array} \rightB =
\leftB \begin{array}{rr}
1 \\
2
\end{array} \rightB
$

\item 
$
\leftB \begin{array}{cc}
a & b \\
c & d
\end{array} \rightB = 
\leftB \begin{array}{cc}
b & c \\
d & a
\end{array} \rightB
$

\end{enumerate}
\begin{sol}
\begin{enumerate}[label={\alph*.}]
\setcounter{enumi}{1}
\item  $(a\ b\ c\ d) = (-2, -4, -6, 0) + t(1, 1, 1, 1)$, \\ $t$ arbitrary

\setcounter{enumi}{3}
\item  $a = b = c = d = t$, $t$ arbitrary

\end{enumerate}
\end{sol}
\end{ex}


\begin{ex}
Compute the following:
\begin{exenumerate}
\exitem*
$
\leftB \begin{array}{rrr}
3 & 2 & 1 \\
5 & 1 & 0
\end{array} \rightB - 5 
\leftB \begin{array}{rrr}
3 & 0 & -2 \\
1 & -1 & 2
\end{array} \rightB
$
\exitem*
$
3 \leftB \begin{array}{r}
3 \\
-1
\end{array} \rightB - 5 
\leftB \begin{array}{r}
6 \\
2
\end{array} \rightB + 7
\leftB \begin{array}{r}
1 \\
-1
\end{array} \rightB
$
\exitem*
$
\leftB \begin{array}{rr}
-2 & 1 \\
3 & 2
\end{array} \rightB - 4 
\leftB \begin{array}{rr}
1 & -2 \\
0 & -1
\end{array} \rightB + 3
\leftB \begin{array}{rr}
2 & -3 \\
-1 & -2
\end{array} \rightB
$
\exitem*
$
\leftB \begin{array}{rrr}
3 & -1 & 2
\end{array} \rightB - 2 
\leftB \begin{array}{rrr}
9 & 3 & 4
\end{array} \rightB +
\leftB \begin{array}{rrr}
3 & 11 & -6
\end{array} \rightB
$
\exitem
$
\leftB \begin{array}{rrrr}
1 & -5 & 4 & 0 \\
2 & 1 & 0 & 6
\end{array} \rightB^{T}
$
\exitem
$
\leftB \begin{array}{rrr}
0 & -1 & 2 \\
1 & 0 & -4 \\
-2 & 4 & 0
\end{array} \rightB^{T}
$ 
\exitem*
$
\leftB \begin{array}{rr}
3 & -1 \\
2 & 1
\end{array} \rightB - 2
\leftB \begin{array}{rr}
1 & -2 \\
1 & 1
\end{array} \rightB^{T}
$
\exitem*
$
3 \leftB \begin{array}{rr}
2 & 1 \\
-1 & 0
\end{array} \rightB^{T} - 2
\leftB \begin{array}{rr}
1 & -1 \\
2 & 3
\end{array} \rightB
$
\end{exenumerate}
\begin{sol}
\begin{enumerate}[label={\alph*.}]
\setcounter{enumi}{1}
\item  
$\leftB \begin{array}{r}
-14 \\
-20
\end{array} \rightB$


\setcounter{enumi}{3}
\item  $(-12, 4, -12)$

\setcounter{enumi}{5}
\item  
$\leftB \begin{array}{rrr}
0 & 1 & -2 \\
-1 & 0 & 4 \\
2 & -4 & 0
\end{array} \rightB$

\setcounter{enumi}{7}
\item  
$\leftB \begin{array}{rr}
4 & -1 \\
-1 & -6
\end{array} \rightB$


\end{enumerate}
\end{sol}
\end{ex}

\begin{ex}
Let 
$A = \leftB \begin{array}{rr}
2 & 1 \\
0 & -1
\end{array} \rightB$, \\ $
B = \leftB \begin{array}{rrr}
3 & -1 & 2 \\
0 & 1 & 4
\end{array} \rightB$,  $
C = \leftB \begin{array}{rr}
3 & -1 \\
2 & 0
\end{array} \rightB$, \\ $
D = \leftB \begin{array}{rr}
1 & 3 \\
-1 & 0 \\
1 & 4
\end{array} \rightB$, and  $ 
E = \leftB \begin{array}{rrr}
1 & 0 & 1 \\
0 & 1 & 0
\end{array} \rightB$.

\noindent Compute the following (where possible).
\begin{exenumerate}
\exitem $3A - 2B$
\exitem $5C$
\exitem $3E^{T}$
\exitem $B + D$
\exitem $4A^{T} - 3C$
\exitem $(A + C)^{T}$
\exitem $2B - 3E$
\exitem $A - D$
\exitem $(B - 2E)^{T}$
\end{exenumerate}
\begin{sol}
\begin{enumerate}[label={\alph*.}]
\setcounter{enumi}{1}
\item  
$\leftB \begin{array}{rr}
15 & -5 \\
10 & 0
\end{array} \rightB$
\setcounter{enumi}{3}
\item  Impossible

\setcounter{enumi}{5}
\item  
$\leftB \begin{array}{rr}
5 & 2 \\
0 & -1
\end{array} \rightB$

\setcounter{enumi}{7}
\item  Impossible

\end{enumerate}
\end{sol}
\end{ex}

\begin{ex}
Find $A$ if:


\begin{enumerate}[label={\alph*.}]
\item 
$
5A - \leftB \begin{array}{rr}
1 & 0 \\
2 & 3
\end{array} \rightB =
3A - \leftB \begin{array}{rr}
5 & 2 \\
6 & 1
\end{array} \rightB
$

\item $
3A - \leftB \begin{array}{r}
2 \\
1
\end{array} \rightB =
5A - 2 \leftB \begin{array}{rr}
3 \\
0
\end{array} \rightB
$

\end{enumerate}
\begin{sol}
\begin{enumerate}[label={\alph*.}]
\setcounter{enumi}{1}
\item  
$\leftB \begin{array}{r}
2 \\
-\frac{1}{2}
\end{array} \rightB$

\end{enumerate}
\end{sol}
\end{ex}

\begin{ex}
Find $A$ in terms of $B$ if:


\begin{exenumerate}
\exitem $A + B = 3A + 2B$
\exitem $2A - B = 5(A + 2B)$
\end{exenumerate}
\begin{sol}
\begin{enumerate}[label={\alph*.}]
\setcounter{enumi}{1}
\item  
$A = -\frac{11}{3}B$

\end{enumerate}
\end{sol}
\end{ex}

\begin{ex}
If $X$, $Y$, $A$, and $B$ are matrices of the same size, solve the following systems of equations to obtain $X$ and $Y$ in terms of $A$ and $B$.
\begin{exenumerate}
\exitem 
$5X + 3Y = A \\
2X + Y = B$
\exitem 
$4X + 3Y = A \\
5X + 4Y = B$
\end{exenumerate}
\begin{sol}
\begin{enumerate}[label={\alph*.}]
\setcounter{enumi}{1}
\item  $X = 4A - 3B$, $Y = 4B - 5A$

\end{enumerate}
\end{sol}
\end{ex}

\begin{ex}
Find all matrices $X$ and $Y$ such that:

\begin{exenumerate}
\exitem $3X - 2Y = \leftB \begin{array}{rr}
3 & - 1 
\end{array} \rightB$
\exitem $2X - 5Y = \leftB \begin{array}{rr}
1 & 2
\end{array} \rightB$
\end{exenumerate}
\begin{sol}
\begin{enumerate}[label={\alph*.}]
\setcounter{enumi}{1}
\item  $Y = (s, t)$, $X = \frac{1}{2}(1 + 5s, 2 + 5t)$; $s$ and $t$ arbitrary

\end{enumerate}
\end{sol}
\end{ex}

\begin{ex}
Simplify the following expressions where $A$, $B$, and $C$ are matrices.

\begin{enumerate}[label={\alph*.}]
\item $2 \leftB 9(A - B) + 7(2B - A) \rightB$ \\ $- 2 \leftB 3(2B + A) - 2(A + 3B) - 5(A + B) \rightB$

\item $5 \leftB 3(A - B + 2C) - 2(3C - B) - A \rightB$  \\ $+ 2 \leftB 3(3A - B + C) + 2(B - 2A) - 2C \rightB$

\end{enumerate}
\begin{sol}
\begin{enumerate}[label={\alph*.}]
\setcounter{enumi}{1}
\item  $20A - 7B + 2C$

\end{enumerate}
\end{sol}
\end{ex}


\begin{ex}
If $A$ is any $2 \times 2$ matrix, show that:


\begin{enumerate}[label={\alph*.}]
\item 
$A = a \leftB \begin{array}{rr}
1 & 0 \\
0 & 0
\end{array} \rightB + 
b \leftB \begin{array}{rr}
0 & 1 \\
0 & 0
\end{array} \rightB + 
c \leftB \begin{array}{rr}
0 & 0 \\
1 & 0
\end{array} \rightB + 
d \leftB \begin{array}{rr}
0 & 0 \\
0 & 1
\end{array} \rightB
$
 for some numbers $a$, $b$, $c$, and $d$.

\item 
$A = p \leftB \begin{array}{rr}
1 & 0 \\
0 & 1
\end{array} \rightB + 
q \leftB \begin{array}{rr}
1 & 1 \\
0 & 0
\end{array} \rightB + 
r \leftB \begin{array}{rr}
1 & 0 \\
1 & 0
\end{array} \rightB + 
s \leftB \begin{array}{rr}
0 & 1 \\
1 & 0
\end{array} \rightB
$
 for some numbers $p$, $q$, $r$, and $s$. 

\end{enumerate}
\begin{sol}
\begin{enumerate}[label={\alph*.}]
\setcounter{enumi}{1}
\item  If 
$A = \leftB \begin{array}{cc}
a & b \\
c & d
\end{array} \rightB$, then $(p, q, r, s) = \frac{1}{2}(2d, a + b - c - d, a - b + c - d, -a + b + c + d)$.

\end{enumerate}
\end{sol}
\end{ex}

\begin{ex}
Let $A = \leftB \begin{array}{rrr}
1 & 1 & -1
\end{array} \rightB$, \\ $B = \leftB \begin{array}{rrr}
0 & 1 & 2
\end{array} \rightB$, and 
$C = \leftB \begin{array}{rrr}
3 & 0 & 1
\end{array} \rightB$. If \\ $rA + sB + tC = 0$ for some scalars $r$, $s$, and $t$, show that necessarily $r = s = t = 0$.
\end{ex}

\begin{ex}
\begin{enumerate}[label={\alph*.}]
\item If $Q + A = A$ holds for every $m \times n$ matrix $A$, show that $Q = 0_{mn}$.

\item If $A$ is an $m \times n$ matrix and $A + A^\prime = 0_{mn}$, show that $A^\prime = -A$.

\end{enumerate}
\begin{sol}
\begin{enumerate}[label={\alph*.}]
\setcounter{enumi}{1}
\item  If $A + A^\prime = 0$ then $-A = -A + 0 = -A + (A + A^\prime) = (-A + A) + A^\prime = 0 + A^\prime = A^\prime$

\end{enumerate}
\end{sol}
\end{ex}

\begin{ex}
If $A$ denotes an $m \times n$ matrix, show that $A = -A$ if and only if $A = 0$.
\end{ex}

\begin{ex}
A square matrix is called a \textbf{diagonal} matrix\index{diagonal matrices}\index{matrix!diagonal matrices} if all the entries off the main diagonal are zero. If $A$ and $B$ are diagonal matrices, show that the following matrices are also diagonal.
\begin{exenumerate}
\exitem $A + B$
\exitem $A - B$
\exitem $kA$ for any number $k$
\end{exenumerate}
\begin{sol}
\begin{enumerate}[label={\alph*.}]
\setcounter{enumi}{1}
\item  Write $A = \diag(a_{1}, \dots, a_{n})$, where $a_{1}, \dots, a_{n}$ are the main diagonal entries. If $B = \diag(b_{1}, \dots, b_{n})$ then $kA = \diag(ka_{1}, \dots, ka_{n})$.

\end{enumerate}
\end{sol}
\end{ex}

\begin{ex}
In each case determine all $s$ and $t$ such that the given matrix is symmetric:
\begin{exenumerate}
\exitem 
$\leftB \begin{array}{rr}
1 & s \\
-2 & t
\end{array} \rightB$
\exitem 
$\leftB \begin{array}{cc}
s & t \\
st & 1
\end{array} \rightB$
\exitem 
$\leftB \begin{array}{crc}
s & 2s & st \\
t & -1 & s \\
t & s^{2} & s
\end{array} \rightB$
\exitem 
$\leftB \begin{array}{ccc}
2 & s & t \\
2s & 0 & s + t \\
3 & 3 & t
\end{array} \rightB$
\end{exenumerate}
\begin{sol}
\begin{enumerate}[label={\alph*.}]
\setcounter{enumi}{1}
\item  $s = 1$ or $t = 0$

\setcounter{enumi}{3}
\item  $s = 0$, and $t = 3$

\end{enumerate}
\end{sol}
\end{ex}

\begin{ex}
In each case find the matrix $A$.


\begin{enumerate}[label={\alph*.}]
\item 
$\left(A + 3 \leftB \begin{array}{rrr}
1 & -1 & 0 \\
1 & 2 & 4
\end{array} \rightB \right)^{T} = \leftB \begin{array}{rr}
2 & 1 \\
0 & 5 \\
3 & 8
\end{array} \rightB$

\item 
$\left(3A^{T} + 2 \leftB \begin{array}{rr}
1 & 0 \\
0 & 2
\end{array} \rightB \right)^{T} = \leftB \begin{array}{rr}
8 & 0 \\
3 & 1
\end{array} \rightB$

\item 
$\left(2A - 3 \leftB \begin{array}{rrr}
1 & 2 & 0
\end{array} \rightB \right)^{T} = 3A^{T} + \leftB \begin{array}{rrr}
2 & 1 & -1
\end{array} \rightB^{T}$ 

\item 
$\left(2A^{T} - 5 \leftB \begin{array}{rr}
1 & 0 \\
-1 & 2
\end{array} \rightB \right)^{T} = 4A - 9 \leftB \begin{array}{rr}
1 & 1 \\
-1 & 0
\end{array} \rightB$

\end{enumerate}
\begin{sol}
\begin{enumerate}[label={\alph*.}]
\setcounter{enumi}{1}
\item  
$\leftB \begin{array}{rr}
2 & 0 \\
1 & -1
\end{array} \rightB$

\setcounter{enumi}{3}
\item  
$\leftB \begin{array}{rr}
2 & 7 \\
-\frac{9}{2} & -5
\end{array} \rightB$


\end{enumerate}
\end{sol}
\end{ex}

\begin{ex}
Let $A$ and $B$ be symmetric (of the same size). Show that each of the following is symmetric.
\begin{exenumerate}
\exitem $(A - B)$
\exitem $kA$ for any scalar $k$
\end{exenumerate}
\begin{sol}
\begin{enumerate}[label={\alph*.}]
\setcounter{enumi}{1}
\item  $A = A^{T}$, so using Theorem~\ref{thm:002240}, $(kA)^{T} = kA^{T} = kA$.

\end{enumerate}
\end{sol}
\end{ex}

\begin{ex}
Show that $A + A^{T}$ is symmetric for \textit{any} square matrix $A$.
\end{ex}

\begin{ex}
If $A$ is a square matrix and $A = kA^{T}$ where $k \neq \pm 1$, show that $A = 0$.
\end{ex}

\begin{ex}
In each case either show that the statement is true or give an example showing it is false.


\begin{enumerate}[label={\alph*.}]
\item If $A + B = A + C$, then $B$ and $C$ have the same size.

\item If $A + B = 0$, then $B = 0$.

\item If the $(3, 1)$-entry of $A$ is $5$, then the $(1, 3)$-entry of $A^{T}$ is $-5$.

\item $A$ and $A^{T}$ have the same main diagonal for every matrix $A$.

\item If $B$ is symmetric and $A^{T} = 3B$, then $A = 3B$.

\item If $A$ and $B$ are symmetric, then $kA + mB$ is symmetric for any scalars $k$ and $m$.

\end{enumerate}
\begin{sol}
\begin{enumerate}[label={\alph*.}]
\setcounter{enumi}{1}
\item  False. Take $B = -A$ for any $A \neq 0$.

\setcounter{enumi}{3}
\item True. Transposing fixes the main diagonal. 

\setcounter{enumi}{5}
\item True. $(kA + mB)^{T} = (kA)^{T} + (mB)^{T} = kA^{T} + mB^{T} = kA + mB$

\end{enumerate}
\end{sol}
\end{ex}


\begin{ex}\label{ex:skewsymmetric}
A square matrix $W$ is called \textbf{skew-symmetric}\index{skew-symmetric}\index{square matrix ($n \times n$ matrix)!skew-symmetric} if $W^{T} = -W$. Let $A$ be any square matrix.


\begin{enumerate}[label={\alph*.}]
\item Show that $A - A^{T}$ is skew-symmetric.

\item Find a symmetric matrix $S$ and a skew-symmetric matrix $W$ such that $A = S + W$.

\item Show that $S$ and $W$ in part (b) are uniquely determined by $A$.

\end{enumerate}
\begin{sol}
\begin{enumerate}[label={\alph*.}]
\setcounter{enumi}{2}
\item  Suppose $A = S + W$, where $S = S^{T}$ and $W = -W^{T}$. Then $A^{T} = S^{T} + W^{T} = S - W$, so $A + A^{T} = 2S$ and $A - A^{T} = 2W$. Hence $S = \frac{1}{2}(A + A^{T})$ and $W = \frac{1}{2}(A - A^{T})$ are uniquely determined by $A$.

\end{enumerate}
\end{sol}
\end{ex}

\begin{ex}
If $W$ is skew-symmetric (Exercise~\ref{ex:skewsymmetric}), show that the entries on the main diagonal are zero. 
\end{ex}

\begin{ex}
Prove the following parts of Theorem~\ref{thm:002170}.
\begin{exenumerate}
\exitem $(k + p)A = kA + pA$
\exitem $(kp)A = k(pA)$
\end{exenumerate}
\begin{sol}
\begin{enumerate}[label={\alph*.}]
\setcounter{enumi}{1}
\item  If $A = \leftB a_{ij} \rightB$ then $(kp)A = \leftB (kp)a_{ij} \rightB = \leftB k(pa_{ij}) \rightB = k \leftB pa_{ij} \rightB = k(pA)$.

\end{enumerate}
\end{sol}
\end{ex}

\begin{ex}
Let $A, A_{1}, A_{2}, \dots, A_{n}$ denote matrices of the same size. Use induction on $n$ to verify the following extensions of properties 5 and 6 of Theorem~\ref{thm:002170}.


\begin{enumerate}[label={\alph*.}]
\item $k(A_{1} + A_{2} + \dots + A_{n}) = kA_{1} + kA_{2} + \dots + kA_{n}$ for any number $k$

\item $(k_{1} + k_{2} + \dots + k_{n})A = k_{1}A + k_{2}A + \dots + k_{n}A$ for any numbers $k_{1}, k_{2}, \dots, k_{n}$

\end{enumerate}
\end{ex}

\begin{ex}
Let $A$ be a square matrix. If $A = pB^{T}$ and $B = qA^{T}$ for some matrix $B$ and numbers $p$ and $q$, show that either $A = 0 = B$ or $pq = 1$. \newline [\textit{Hint}: Example~\ref{exa:002159}.]
\end{ex}

\end{multicols}
